\documentclass[fleqn]{article}

\usepackage{amsmath}
\usepackage[top=2mm, bottom=2mm, left=2mm, right=30mm]{geometry}
\begin{document}

This is to complement the part of the solution about finding the probability at all in points.

First, because it is an all in point, if we lose, we are done so the equation reduces to just

\begin{equation}
\begin{alignedat}{2}
  P_y  = && p * P_{2y} + (1-p) * P_{0}  \\
   P_y  = && p * P_{2y} 
 \end{alignedat}
\end{equation}


Given x is amt of money, and P is probability of winning / getting to V

From one all in point to the next

Make a line from $ (i, P_i) $  to $ (k, P_k) $ since it is linear.

where i is the all in point we are calculating $P_i$.

Let $ j = 2 * i $ and $ P_i = p * P_j $

To start off $k, P_k$ is the final state $(V, 1)$ afterwards, it will be the last all in point calculated.
That means $k, P_k, i, j, k, p$ are all known, we are looking for $P_i$ and $P_j$.

$p$ is calculated from $p = \frac{A-L}{V-L}$ or in this case $p = \frac{i-L}{j-L}$

L is given by $-2i * (2^\text{infnum} - 1)$

Goal is to get $P_i$ and $P_j$ on left side


\begin{equation}
\begin{alignedat}{2}
  P - P_k  = && \frac{P_k-P_i}{k-i} * (x - k)   \\
  P_j - P_k  = && \frac{P_k-P_i}{k-i} * (j - k)   \\
  (P_j - P_k) * (k-i) =  && (P_k-P_i) * (j - k) \\
  P_j * (k-i) - P_k * (k-i)  = && P_k * (j-k) - P_i * (j -k ) \\
  P_j * (k-i)  + P_i * (j -k ) = && P_k * (j-k)  + P_k * (k-i)\\
  P_j * (k-i)  + p*P_j * (j -k ) = && P_k * (j-k)  + P_k * (k-i)\\
  P_j  = && \frac{P_k * ( (j-k)  + (k-i)} {(k-i)+p*(j-k)}\\
  P_j  = && \frac{P_k * ( j-i)} {(k-i)+p*(j-k)}\\
  a = b
 \end{alignedat}
\end{equation}


\end{document}
